coq/assoc_spec.v
@@ -1,15 +1,15 @@
 Require Import Coq.ZArith.Zbool.
 Require Import Coq.ZArith.BinInt.
 Require Import ZArith.ZArith_dec.
+Require Import ZArith.ZArith_base.
+Require Import ZArith.Zdiv.
 Require Import Coq.Setoids.Setoid.
 
-Local Open Scope Z_scope.
-(*Local Open Scope Z.*)
-Locate Z.
+Local Open Scope Z.
 
 Definition ArrayZ := Z->Z.
 
-Function arrPut (arr: ArrayZ) (k:Z) (v:Z) : Z -> Z :=
+Function arrPut (arr: ArrayZ) (k:Z) (v:Z) : ArrayZ :=
   fun (kk:Z) => if (Z.eq_dec k kk) then v else arr kk.
 
 Function arrGet (arr: ArrayZ) (k:Z) : Z :=
@@ -28,5 +28,30 @@ Proof.
 intros.
 unfold arrGet, arrPut.
 destruct Z.eq_dec;[contradiction|tauto].
+Qed.
+
+Definition CircleArrayZ := ArrayZ.
+
+Function caPut (arr: CircleArrayZ) (k:Z) (v:Z) : CircleArrayZ :=
+  arrPut arr (Zmod k 100) v.
+
+Function caGet (arr:CircleArrayZ) (k:Z) : Z :=
+  arrGet arr (Zmod k 100).
+
+Lemma Cgetput1: forall arr k v, caGet (caPut arr k v) k = v.
+Proof.
+intros.
+unfold caGet, caPut.
+apply getput1.
+Qed.
+
+Lemma Cgetput2: forall arr k1 k2 v2, k2 mod 100 <> k1 mod 100 -> 
+                                     caGet (caPut arr k2 v2) k1 =
+                                     caGet arr k1.
+Proof.
+intros.
+unfold caGet, caPut.
+apply getput2.
+assumption.
 Qed.
 
